src/MicroSail/Environment.v
@@ -5,9 +5,9 @@ Require Import MicroSail.Notation.
 Set Implicit Arguments.
 
 Section WithBinding.
-  Context {B : Set}.
+  Context {B : Type}.
 
-  Inductive Env (D : B -> Set) : Ctx B -> Set :=
+  Inductive Env (D : B -> Type) : Ctx B -> Type :=
   | env_nil : Env D ctx_nil
   | env_snoc {Γ} (E : Env D Γ) (b : B) (db : D b) :
       Env D (ctx_snoc Γ b).
@@ -15,21 +15,21 @@ Section WithBinding.
   Global Arguments env_nil {_}.
   Bind Scope env_scope with Env.
 
-  Fixpoint env_cat {D : B -> Set} {Γ Δ : Ctx B}
+  Fixpoint env_cat {D : B -> Type} {Γ Δ : Ctx B}
     (EΓ : Env D Γ) (EΔ : Env D Δ) : Env D (ctx_cat Γ Δ) :=
     match EΔ with
     | env_nil => EΓ
     | env_snoc E b db => env_snoc (env_cat EΓ E) b db
     end.
 
-  Fixpoint env_map {D1 D2 : B -> Set} {Γ : Ctx B}
+  Fixpoint env_map {D1 D2 : B -> Type} {Γ : Ctx B}
     (f : forall b, D1 b -> D2 b) (E : Env D1 Γ) : Env D2 Γ :=
     match E with
     | env_nil => env_nil
     | env_snoc E b db => env_snoc (env_map f E) b (f b db)
     end.
 
-  Fixpoint env_lookup {D : B -> Set} {Γ : Ctx B}
+  Fixpoint env_lookup {D : B -> Type} {Γ : Ctx B}
     (E : Env D Γ) : forall (b : B) (bIn : InCtx b Γ), D b :=
     match E with
     | env_nil => fun _ => inctx_case_nil
@@ -38,7 +38,7 @@ Section WithBinding.
 
   Global Arguments env_lookup {_ _} _ [_] _.
 
-  Fixpoint env_update {D : B -> Set} {Γ : Ctx B} (E : Env D Γ) {struct E} :
+  Fixpoint env_update {D : B -> Type} {Γ : Ctx B} (E : Env D Γ) {struct E} :
     forall {b0 : B} (bIn0 : InCtx b0 Γ) (new : D b0), Env D Γ :=
     match E with
     | env_nil => fun _ => inctx_case_nil
@@ -49,7 +49,7 @@ Section WithBinding.
         (fun b0' bIn0' new => env_snoc (env_update E bIn0' new) b bold)
     end.
 
-  Definition env_tail {D : B -> Set} {Γ : Ctx B}
+  Definition env_tail {D : B -> Type} {Γ : Ctx B}
     {b : B} (E : Env D (ctx_snoc Γ b)) : Env D Γ :=
     match E in Env _ Γb
     return match Γb with
@@ -63,14 +63,14 @@ Section WithBinding.
 
   Global Arguments env_tail {_ _ _} / _.
 
-  Fixpoint env_drop {D : B -> Set} {Γ : Ctx B} Δ {struct Δ} :
+  Fixpoint env_drop {D : B -> Type} {Γ : Ctx B} Δ {struct Δ} :
     forall (E : Env D (ctx_cat Γ Δ)), Env D Γ :=
     match Δ with
     | ctx_nil => fun E => E
     | ctx_snoc Δ _ => fun E => env_drop Δ (env_tail E)
     end.
 
-  Fixpoint env_split {D : B -> Set} {Γ : Ctx B} Δ {struct Δ} :
+  Fixpoint env_split {D : B -> Type} {Γ : Ctx B} Δ {struct Δ} :
     forall (E : Env D (ctx_cat Γ Δ)), Env D Γ * Env D Δ :=
     match Δ with
     | ctx_nil => fun E => (E , env_nil)
@@ -89,7 +89,7 @@ Section WithBinding.
         end (env_split Δ)
     end.
 
-  Lemma env_lookup_update {D : B -> Set} {Γ : Ctx B} (E : Env D Γ) :
+  Lemma env_lookup_update {D : B -> Type} {Γ : Ctx B} (E : Env D Γ) :
     forall {b : B} (bInΓ : InCtx b Γ) (db : D b),
       env_lookup (env_update E bInΓ db) bInΓ = db.
   Proof.
@@ -97,12 +97,12 @@ Section WithBinding.
       destruct n; cbn in *; subst; auto.
   Qed.
 
-  Lemma env_split_cat {D : B -> Set} {Γ Δ : Ctx B} :
+  Lemma env_split_cat {D : B -> Type} {Γ Δ : Ctx B} :
     forall (EΓ : Env D Γ) (EΔ : Env D Δ),
       env_split Δ (env_cat EΓ EΔ) = (EΓ , EΔ).
   Proof. induction EΔ using Env_ind; cbn; now try rewrite IHEΔ. Qed.
 
-  Lemma env_cat_split' {D : B -> Set} {Γ Δ : Ctx B} :
+  Lemma env_cat_split' {D : B -> Type} {Γ Δ : Ctx B} :
     forall (EΓΔ : Env D (ctx_cat Γ Δ)),
       let (EΓ,EΔ) := env_split _ EΓΔ in
       EΓΔ = env_cat EΓ EΔ.
@@ -114,21 +114,21 @@ Section WithBinding.
       destruct (env_split Δ EΓΔ); now subst.
   Qed.
 
-  Lemma env_cat_split {D : B -> Set} {Γ Δ : Ctx B} (EΓΔ : Env D (ctx_cat Γ Δ)) :
+  Lemma env_cat_split {D : B -> Type} {Γ Δ : Ctx B} (EΓΔ : Env D (ctx_cat Γ Δ)) :
     EΓΔ = env_cat (fst (env_split _ EΓΔ)) (snd (env_split _ EΓΔ)).
   Proof.
     generalize (env_cat_split' EΓΔ).
     now destruct (env_split Δ EΓΔ).
   Qed.
 
-  Lemma env_drop_cat {D : B -> Set} {Γ Δ : Ctx B} :
+  Lemma env_drop_cat {D : B -> Type} {Γ Δ : Ctx B} :
     forall (δΔ : Env D Δ) (δΓ : Env D Γ),
       env_drop Δ (env_cat δΓ δΔ) = δΓ.
   Proof. induction δΔ; cbn; auto. Qed.
 
 End WithBinding.
 
-Definition Env' {X T : Set} (D : T -> Set) (Γ : Ctx (X * T)) : Set :=
+Definition Env' {X T : Set} (D : T -> Type) (Γ : Ctx (X * T)) : Type :=
   Env (fun xt => D (snd xt)) Γ.
 Bind Scope env_scope with Env.
 Bind Scope env_scope with Env'.
